readme.md
@@ -3,7 +3,7 @@
 Pipit is an embedded language for implementing and verifying *reactive systems*, such as the anti-lock braking system in a car, or the  [system that fills the water reservoir of your coffee machine](https://youtu.be/6IybbQFPOl8).
 Pipit is a research project and is in the early stages of development.
 
-Pipit is implemented in  [F*](https://www.fstar-lang.org/).
+Pipit is implemented in  [F\*](https://www.fstar-lang.org/).
 The language is strongly inspired by Lustre.
 The verification system is inspired by the [Kind2 model checker](https://github.com/kind2-mc/kind2/) and related work.
 By embedding Pipit in a theorem prover, we aim to have an expressive language with a small verifiable core.
@@ -39,54 +39,48 @@ Make sure you have [opam](https://opam.ocaml.org/) installed.
 Run this from the Pipit directory:
 
 ``` sh
-# Create a directory for the build environment
-mkdir -p build/env; cd build/env
-
 # Create a local opam switch with OCaml 4.14
 opam switch create . 4.14.1
 
-# git clone https://github.com/FStarLang/karamel
-
-# Is it necessary to check out a specific commit of F*?
-# git clone https://github.com/FStarLang/FStar
-# cd FStar; git checkout 5a15885098c69006bb56ff2712534fe75a5fd839; cd ..
-
-# Tell opam to use the development version of F* (but don't install it yet)
+# Tell opam to use the development version of F* but don't install it yet
 opam pin add fstar --dev-repo --no-action
 
-# Tell opam where to find the local repo for Karamel (and install it and F*)
+# Tell opam where to find the local repo for Karamel and install it and F*
 opam pin add karamel --dev-repo --yes
 ```
 
 ### IDE configuration
 
-When using an IDE (Emacs, VSCode), you might need to specify the exact version of FStar and Z3 binaries to use.
+When using an IDE (Emacs, VSCode), you probably need to specify the exact version of FStar and Z3 binaries to use.
 
 
 #### VSCode
 
 There are a few VSCode extensions that provide different levels of F\* support; you should use [fstar-vscode-assistant](https://marketplace.visualstudio.com/items?itemName=FStarLang.fstar-vscode-assistant).
 
-You may need to tell VSCode the path of your F\* installation.
-Copy `template.fst.config.json` to `.fst.config.json` and modify it to include the path to `fstar.exe` as necessary.
-
-If you have multiple versions of Z3 installed, you will probably also have to specify the path to the F\*-compatible Z3 with the `--smt /.../bin/z3` option.
-For example, my `.fst.config.json` is:
-
-```json
-{ "fstar_exe":"/Users/amos/proj/ext/fstar/_opam/bin/fstar.exe",
-  "options":["--smt", "/Users/amos/proj/ext/fstar/_opam/bin/z3", "--cache_dir", ".cache.boot"],
-  "include_dirs":["src","example"]
-}
-```
+If you are using a local `opam` switch, as described above, you may will to tell VSCode the path of your F\* installation.
+Copy `template.fst.config.json` to `.fst.config.json`.
 
 #### Emacs
 
-Emacs
+To set up Emacs to use the local `opam` switch, I modified the global fstar options in Emacs.
+I modified my `~/.doom.d/config.el` to include:
 
 ``` emacs-lisp
 (setq-default
-  fstar-executable "/Users/amos/proj/ext/fstar/_opam/bin/fstar.exe"
-  fstar-smt-executable "/Users/amos/proj/ext/fstar/_opam/bin/z3")
+  fstar-executable "/Users/amos/proj/songlark/pipit/_opam/bin/fstar.exe"
+  fstar-smt-executable "/Users/amos/proj/songlark/pipit/_opam/bin/z3"
+  fstar-subp-prover-args
+  '("--include" "/Users/amos/proj/songlark/pipit/src"
+    "--include" "/Users/amos/proj/songlark/pipit/example"
+    "--cache_dir" "/Users/amos/proj/songlark/pipit/build/cache"))
 ```
+
+(Is it easy to set project-local options in Emacs? It would be convenient if the Emacs fstar-mode read `.fst.config.json` too.)
+
+## Build instructions
+
+Use `make verify` to check the proofs.
+Use `make extract` to extract C code for the Pump example; the extracted C code is written to `build/extract`.
+The embedded system that actually runs the Pump example is in the [app-pipit-pump repository](https://github.com/songlarknet/app-pipit-pump); it uses the Zephyr RTOS.
 
